simple-frontend/FrontEndTranslation.thy
@@ -4,159 +4,967 @@ begin
 
 type_synonym v_stmt = "(int equi_state, int val, int custom) abs_stmt"
 
+definition semantify_exp :: "ParImp.exp \<Rightarrow> (int equi_state, int val) AbstractSemantics.exp" where
+  "semantify_exp e \<omega> = Some (VInt (edenot e (get_store \<omega>)))"
+
+definition semantify_bexp :: "ParImp.bexp \<Rightarrow> (int equi_state) AbstractSemantics.bexp" where
+  "semantify_bexp b \<omega> = (if (bdenot b (get_store \<omega>)) then Some True else Some False)"
+
+definition semantify_addr :: "var \<Rightarrow> (int equi_state, address) AbstractSemantics.exp" where
+  "semantify_addr x \<omega> = (if (\<exists>l. get_store \<omega> x = Some (VRef (Address l)))
+  then Some (SOME l. get_store \<omega> x = Some (VRef (Address l)))
+  else None)"
+
+lemma semantify_addr_equiv:
+  "semantify_addr x \<omega> = Some l \<longleftrightarrow> get_store \<omega> x = Some (VRef (Address l))"
+  using semantify_addr_def by auto
+
+lemma convert_proof_assign:
+  assumes "ConcreteSemantics.SL_proof \<Delta> A (abs_stmt.LocalAssign x (semantify_exp e)) B"
+  shows "\<Delta> \<turnstile>CSL [A] Cassign x e [B]"
+proof -
+  have "B = ConcreteSemantics.post_substitute_var_assert x (semantify_exp e) A"
+    using ConcreteSemantics.SL_proof_LocalAssign_elim assms
+    by fast
+  moreover have "\<Delta> \<turnstile>CSL [A] Cassign x e [ConcreteSemantics.post_substitute_var_assert x (semantify_exp e) A]"
+  proof (rule RuleCons)
+    show "A \<subseteq> sub_pre x e (ConcreteSemantics.post_substitute_var_assert x (semantify_exp e) A)"
+      unfolding sub_pre_def ConcreteSemantics.post_substitute_var_assert_def ConcreteSemantics.substitute_var_state_def TypedEqui.assign_var_state_def
+    proof (clarify)
+      fix a aa b
+      assume asm0: "(a, aa, b) \<in> A"
+      moreover have "a = Ag (the_ag a)" by simp
+      moreover have "(Ag ((the_ag a)(x \<mapsto> VInt (edenot e (the_ag a)))), aa, b) \<in> (\<lambda>\<omega>. set_store \<omega> ((get_store \<omega>)(x := semantify_exp e \<omega>))) ` A"
+        by (metis (no_types, lifting) ConcreteSemantics.set_store_Ag_simplies asm0 calculation(2) get_simps_unfolded(1) image_iff semantify_exp_def)
+      ultimately show "\<exists>s \<tau> \<omega>. (a, aa, b) = (Ag s, \<tau>, \<omega>) \<and> (Ag (s(x \<mapsto> VInt (edenot e s))), \<tau>, \<omega>) \<in> (\<lambda>\<omega>. set_store \<omega> ((get_store \<omega>)(x := semantify_exp e \<omega>))) ` A"
+        by blast
+    qed
+    show "\<Delta> \<turnstile>CSL [sub_pre x e (ConcreteSemantics.post_substitute_var_assert x (semantify_exp e) A)] Cassign x e [ConcreteSemantics.post_substitute_var_assert x (semantify_exp e) A]"
+      by (simp add: RuleAssign)
+  qed (simp)
+  ultimately show ?thesis by auto
+qed
+
+lemma convert_proof_skip:
+  assumes "ConcreteSemantics.SL_proof \<Delta> A Skip B"
+  shows "\<Delta> \<turnstile>CSL [A] Cskip [B]"
+  using RuleSkip assms by blast
+
+lemma conjunct_with_true_entails:
+  assumes "TypedEqui.typed_assertion \<Delta> P"
+  shows "P \<subseteq> atrue \<Delta> \<otimes> P"
+proof
+  fix \<omega> assume "\<omega> \<in> P"
+  then have "Some \<omega> = |\<omega>| \<oplus> \<omega>"
+    by (simp add: commutative core_is_smaller)
+  moreover have "|\<omega>| \<in> atrue \<Delta>"
+    by (metis CollectI TypedEqui.typed_core TypedEqui.typed_state_axioms \<open>\<omega> \<in> P\<close> assms atrue_def typed_state.typed_assertionE)
+  ultimately show "\<omega> \<in> atrue \<Delta> \<otimes> P"
+    using \<open>\<omega> \<in> P\<close> x_elem_set_product by blast
+qed
+
+
+fun wf_stmt where
+  "wf_stmt \<Delta> (Cseq C1 C2) \<longleftrightarrow> wf_stmt \<Delta> C1 \<and> wf_stmt \<Delta> C2"
+| "wf_stmt \<Delta> (Calloc r e) \<longleftrightarrow> r \<notin> fvE e"
+| "wf_stmt \<Delta> ({P1} C1 {Q1} || {P2} C2 {Q2}) \<longleftrightarrow>
+  disjoint (fvC C1 \<union> fvA \<Delta> (Q1 \<otimes> atrue \<Delta>)) (wrC C2) \<and> disjoint (fvC C2 \<union> fvA \<Delta> (Q2 \<otimes> atrue \<Delta>)) (wrC C1) \<and>
+  TypedEqui.self_framing_typed \<Delta> P1 \<and> TypedEqui.typed_assertion \<Delta> P1 \<and>
+  TypedEqui.self_framing_typed \<Delta> P2 \<and> TypedEqui.typed_assertion \<Delta> P2 \<and>
+  wf_stmt \<Delta> C1 \<and> wf_stmt \<Delta> C2"
+| "wf_stmt \<Delta> (Cif b C1 C2) \<longleftrightarrow> wf_stmt \<Delta> C1 \<and> wf_stmt \<Delta> C2"
+
+| "wf_stmt \<Delta> _ \<longleftrightarrow> True"
+
+lemma fvA_charact_exists:
+  "fvA \<Delta> (TypedEqui.exists_assert \<Delta> r P) \<subseteq> fvA \<Delta> P - {r}"
+  sorry (* fvA \<Delta> *)
+
+lemma fvaA_atrue_empty[simp]:
+  "fvA \<Delta> (atrue \<Delta>) = {}"
+  sorry (* fvA \<Delta> *)
+
+lemma atrue_self_framing_and_typed[simp]:
+  "TypedEqui.typed_assertion \<Delta> (atrue \<Delta>)"
+  "TypedEqui.self_framing_typed \<Delta> (atrue \<Delta>)"
+  using TypedEqui.typed_assertionI atrue_def apply blast
+  by (simp add: TypedEqui.self_framing_typedI TypedEqui.typed_state_then_stabilize_typed atrue_def)
+
+lemma convert_proof_alloc:
+  assumes "ConcreteSemantics.SL_proof \<Delta> P (Havoc r;; Inhale (full_ownership_with_val r e)) Q"
+      and "well_typed_cmd \<Delta> (Calloc r e)"
+      and "wf_stmt \<Delta> (Calloc r e)"
+  shows "\<Delta> \<turnstile>CSL [P] Calloc r e [Q]"
+proof (rule RuleCons)
+
+  have asm0: "ConcreteSemantics.SL_proof \<Delta> P (Havoc r) (TypedEqui.exists_assert \<Delta> r P)
+  \<and> ConcreteSemantics.SL_proof \<Delta> (TypedEqui.exists_assert \<Delta> r P) (Inhale (full_ownership_with_val r e)) Q
+  \<and> TypedEqui.self_framing_typed \<Delta> P"
+    by (metis ConcreteSemantics.SL_proof_Havoc_elim ConcreteSemantics.SL_proof_Seq_elim assms(1))
+  then have "Q = TypedEqui.exists_assert \<Delta> r P \<otimes> full_ownership_with_val r e"
+    by blast
+
+  show "\<Delta> \<turnstile>CSL [atrue \<Delta> \<otimes> TypedEqui.exists_assert \<Delta> r P] Calloc r e [full_ownership_with_val r e \<otimes> TypedEqui.exists_assert \<Delta> r P]"
+  proof (rule RuleFrame)
+    have "r \<notin> fvE e"
+      using assms(3) by auto
+    then show "\<Delta> \<turnstile>CSL [atrue \<Delta>] Calloc r e [full_ownership_with_val r e]"
+      using RuleAlloc[of r e] by simp
+    show "disjoint (fvA \<Delta> (TypedEqui.exists_assert \<Delta> r P)) (wrC (Calloc r e))"
+      by (metis (no_types, opaque_lifting) Diff_iff Diff_insert_absorb disjoint_minus disjoint_simps(1) ex_in_conv fvA_charact_exists subset_Diff_insert wrC.simps(5))
+    show "TypedEqui.self_framing_typed \<Delta> (atrue \<Delta>)"
+      using TypedEqui.self_framing_typed_def atrue_def
+      using TypedEqui.typed_state_then_stabilize_typed by blast
+    show "TypedEqui.self_framing_typed \<Delta> (TypedEqui.exists_assert \<Delta> r P)"
+      using asm0 by fastforce
+    show "TypedEqui.typed_assertion \<Delta> (TypedEqui.exists_assert \<Delta> r P)"
+      using asm0 by fastforce
+    show "TypedEqui.typed_assertion \<Delta> (atrue \<Delta>)"
+      using TypedEqui.typed_assertion_def atrue_def by blast
+  qed
+
+  moreover have "TypedEqui.typed_assertion \<Delta> P \<and> variables \<Delta> r \<noteq> None"
+  proof
+    show "TypedEqui.typed_assertion \<Delta> P"
+      using asm0 by blast
+    show "variables \<Delta> r \<noteq> None"
+      using assms(2) by auto
+  qed
+  then have "entails P (TypedEqui.exists_assert \<Delta> r P)"
+    using ConcreteSemantics.SL_proof_Havoc_elim_entails[of \<Delta> P r "TypedEqui.exists_assert \<Delta> r P"]    
+    using ConcreteSemantics.exists_assert_entails by blast
+
+  then show "P \<subseteq> atrue \<Delta> \<otimes> TypedEqui.exists_assert \<Delta> r P"
+    by (meson TypedEqui.typed_assertion_exists_assert \<open>TypedEqui.typed_assertion \<Delta> P \<and> variables \<Delta> r \<noteq> None\<close> conjunct_with_true_entails dual_order.trans entails_def)
+  show "full_ownership_with_val r e \<otimes> TypedEqui.exists_assert \<Delta> r P \<subseteq> Q"
+    by (simp add: \<open>Q = TypedEqui.exists_assert \<Delta> r P \<otimes> full_ownership_with_val r e\<close> add_set_commm)
+qed
+
+lemma helper_exhale_encoding:
+  assumes "ConcreteSemantics.SL_proof \<Delta> P (Exhale (Stabilize A)) Q"
+  shows "P \<subseteq> TypedEqui.Stabilize_typed \<Delta> A \<otimes> Q"
+  using assms(1)
+proof (rule ConcreteSemantics.SL_proof_Exhale_elim)
+  assume asm0: "entails P (Q \<otimes> Stabilize A)" "TypedEqui.self_framing_typed \<Delta> P"
+    "TypedEqui.typed_assertion \<Delta> P" "TypedEqui.self_framing_typed \<Delta> Q"
+    "TypedEqui.typed_assertion \<Delta> Q"
+  show "P \<subseteq> TypedEqui.Stabilize_typed \<Delta> A \<otimes> Q"
+  proof
+    fix \<omega> assume asm1: "\<omega> \<in> P"
+    then obtain q a where "q \<in> Q" "a \<in> Stabilize A" "Some \<omega> = q \<oplus> a"
+      by (meson asm0(1) entails_def subsetD x_elem_set_product)
+    moreover have "TypedEqui.typed \<Delta> a"
+      using TypedEqui.typed_state_axioms asm0(3) asm1 calculation(3) greater_equiv typed_state.typed_assertionE typed_state.typed_smaller by blast
+    then have "stabilize a \<in> A"
+      using calculation(2) by auto
+    thm TypedEqui.Stabilize_typed_def Stabilize_def
+
+    then show "\<omega> \<in> TypedEqui.Stabilize_typed \<Delta> A \<otimes> Q"
+      by (metis (no_types, lifting) ConcreteSemantics.stabilize_typed_elem \<open>TypedEqui.typed \<Delta> a\<close> calculation(1) calculation(3) commutative x_elem_set_product)
+  qed
+qed
+
+lemma convert_proof_free:
+  assumes "ConcreteSemantics.SL_proof \<Delta> P (Exhale (Stabilize (full_ownership r))) Q"
+  shows "\<Delta> \<turnstile>CSL [P] Cfree r [Q \<otimes> atrue \<Delta>]"
+  using assms(1)
+proof (rule ConcreteSemantics.SL_proof_Exhale_elim)
+  assume asm0: "entails P (Q \<otimes> Stabilize (full_ownership r))" "TypedEqui.self_framing_typed \<Delta> P"
+    "TypedEqui.typed_assertion \<Delta> P" "TypedEqui.self_framing_typed \<Delta> Q" "TypedEqui.typed_assertion \<Delta> Q"
+  show "\<Delta> \<turnstile>CSL [P] Cfree r [Q \<otimes> atrue \<Delta>]"
+  proof (rule RuleCons)
+    show "\<Delta> \<turnstile>CSL [TypedEqui.Stabilize_typed \<Delta> (full_ownership r) \<otimes> Q] Cfree r [TypedEqui.Stabilize_typed \<Delta> (atrue \<Delta>) \<otimes> Q]"
+    proof (rule RuleFrame)
+      show "\<Delta> \<turnstile>CSL [TypedEqui.Stabilize_typed \<Delta> (full_ownership r)] Cfree r [TypedEqui.Stabilize_typed \<Delta> (atrue \<Delta>)]"
+        by (simp add: RuleFree RuleStabilizeTyped)
+    qed (simp_all add: asm0)
+    show "P \<subseteq> TypedEqui.Stabilize_typed \<Delta> (full_ownership r) \<otimes> Q"
+      by (simp add: assms helper_exhale_encoding)
+    show "TypedEqui.Stabilize_typed \<Delta> (atrue \<Delta>) \<otimes> Q \<subseteq> Q \<otimes> atrue \<Delta>"
+      by (metis TypedEqui.typed_Stabilize_typed TypedEqui.typed_assertion_def add_set_commm add_set_mono atrue_def mem_Collect_eq subsetI)
+  qed
+qed
+
+lemma in_Stabilize_typed:
+  assumes "stabilize \<omega> \<in> A"
+      and "TypedEqui.typed \<Delta> \<omega>"
+    shows "\<omega> \<in> TypedEqui.Stabilize_typed \<Delta> A"
+  using ConcreteSemantics.stabilize_typed_elem assms(1) assms(2) by blast
+
+
+lemma larger_mask_full:
+  assumes "\<omega>' \<succeq> \<omega>"
+      and "get_m \<omega> l = 1"
+    shows "get_m \<omega>' l = 1"
+  by (metis (no_types, lifting) assms(1) assms(2) get_m_additive get_vm_bound greater_def nle_le pos_perm_class.sum_larger)
+
+lemma greater_equiI:
+  assumes "get_m a \<succeq> get_m b"
+      and "get_h a \<succeq> get_h b"
+      and "get_store a = get_store b"
+      and "get_trace a = get_trace b"
+    shows "a \<succeq> b"
+  apply (rule greater_prodI)
+   apply (metis ag_store_greater agreement.exhaust_sel assms(3) get_store_def)
+  apply (rule greater_prodI)
+  apply (metis assms(4) fst_conv greater_Ag set_state_def set_state_get_state snd_conv)
+proof -
+  have "Rep_virtual_state (snd (snd a)) \<succeq> Rep_virtual_state (snd (snd b))"
+    by (metis assms(1) assms(2) get_state_def get_vh_def get_vm_def greater_prodI)
+  then show "snd (snd a) \<succeq> snd (snd b)"
+    using wf_greater_preserve
+    by (metis Rep_virtual_state_inverse get_vh_def get_vm_def vstate_wf_ppos wf_mask_simple_get_vm wf_pre_virtual_state_def)
+qed
+
+
+lemma in_times_atrue:
+  assumes "TypedEqui.typed \<Delta> \<omega>'"
+      and "\<omega>' \<succeq> \<omega>"
+      and "\<omega> \<in> A"
+    shows "\<omega>' \<in> A \<otimes> atrue \<Delta>"
+proof -
+  obtain r where "Some \<omega>' = \<omega> \<oplus> r"
+    using assms(2) greater_def by blast
+  then have "r \<in> atrue \<Delta>"
+    using TypedEqui.typed_smaller assms(1) atrue_def greater_equiv by blast
+  then show ?thesis
+    using \<open>Some \<omega>' = \<omega> \<oplus> r\<close> assms(3) x_elem_set_product by blast
+qed
+
+lemma convert_proof_write:
+  assumes "ConcreteSemantics.SL_proof \<Delta> P (Custom (FieldAssign (semantify_addr r) field_val (semantify_exp e))) Q"
+  shows "\<Delta> \<turnstile>CSL [P] Cwrite r e [Q \<otimes> atrue \<Delta>]"
+  using assms(1)
+proof (rule ConcreteSemantics.SL_proof_Custom_elim)
+  assume asm0: "SL_Custom \<Delta> P (custom.FieldAssign (semantify_addr r) field_val (semantify_exp e)) Q"
+  "TypedEqui.self_framing_typed \<Delta> P" "TypedEqui.typed_assertion \<Delta> P" "TypedEqui.self_framing_typed \<Delta> Q"
+  "TypedEqui.typed_assertion \<Delta> Q"
+  show "\<Delta> \<turnstile>CSL [P] Cwrite r e [Q \<otimes> atrue \<Delta>]"
+    using asm0(1)
+  proof (rule SL_custom_FieldAssign)
+    assume asm1: "Q = update_value \<Delta> P (semantify_addr r) field_val (semantify_exp e)"
+      "TypedEqui.self_framing_typed \<Delta> P" "entails P {\<omega>. \<exists>l. get_m \<omega> (l, field_val) = 1 \<and> semantify_addr r \<omega> = Some l}"
+      "framed_by_exp P (semantify_addr r)" "framed_by_exp P (semantify_exp e)"
+    show "\<Delta> \<turnstile>CSL [P] Cwrite r e [Q \<otimes> atrue \<Delta>]"
+    proof (rule RuleCons)
+      let ?F = "TypedEqui.Stabilize_typed \<Delta> { remove_only \<omega> (l, field_val) |\<omega> l. \<omega> \<in> P \<and> semantify_addr r \<omega> = Some l}"
+      show "\<Delta> \<turnstile>CSL [TypedEqui.Stabilize_typed \<Delta> (full_ownership r) \<otimes> ?F] Cwrite r e [TypedEqui.Stabilize_typed \<Delta> (full_ownership_with_val r e) \<otimes> ?F]"
+      proof (rule RuleFrame)
+        show "\<Delta> \<turnstile>CSL [TypedEqui.Stabilize_typed \<Delta> (full_ownership r)] Cwrite r e [TypedEqui.Stabilize_typed \<Delta> (full_ownership_with_val r e)]"
+          by (simp add: RuleStabilizeTyped RuleWrite)
+      qed (simp_all)
+      show "P \<subseteq> TypedEqui.Stabilize_typed \<Delta> (full_ownership r) \<otimes> ?F"
+      proof
+        fix \<omega> assume "\<omega> \<in> P"
+        then obtain l where "get_m \<omega> (l, field_val) = 1 \<and> semantify_addr r \<omega> = Some l"          
+          by (smt (verit) CollectD asm1(3) entails_def subsetD)
+        then have "Some \<omega> = remove_only \<omega> (l, field_val) \<oplus> set_state \<omega> (Abs_virtual_state (concretize (\<lambda>l'. if (l, field_val) = l' then 1 else 0) (get_state \<omega>)))"
+          using split_remove_only_owns_only by blast
+        moreover have "set_state \<omega> (Abs_virtual_state (concretize (\<lambda>l'. if (l, field_val) = l' then 1 else 0) (get_state \<omega>))) \<in> TypedEqui.Stabilize_typed \<Delta> (full_ownership r)"
+        proof (rule in_Stabilize_typed)
+          show "TypedEqui.typed \<Delta> (set_state \<omega> (Abs_virtual_state (concretize (\<lambda>l'. if (l, field_val) = l' then 1 else 0) (get_state \<omega>))))"
+            using TypedEqui.typed_state_axioms \<open>\<omega> \<in> P\<close> asm0(3) calculation greater_equiv typed_state.typed_assertionE typed_state.typed_smaller by blast
+          show "stabilize (set_state \<omega> (Abs_virtual_state (concretize (\<lambda>l'. if (l, field_val) = l' then 1 else 0) (get_state \<omega>)))) \<in> full_ownership r"
+            apply (rule in_full_ownership[of _ _ l])
+            using \<open>get_m \<omega> (l, field_val) = 1 \<and> semantify_addr r \<omega> = Some l\<close> semantify_addr_equiv apply auto[1]
+            by (smt (verit, best) \<open>get_m \<omega> (l, field_val) = 1 \<and> semantify_addr r \<omega> = Some l\<close> add.commute add.right_neutral calculation fun_upd_apply get_m_additive get_m_stabilize remove_only_charact(2))
+        qed
+        moreover have "remove_only \<omega> (l, field_val) \<in> ?F"
+        proof (rule in_Stabilize_typed)
+          have "stabilize (remove_only \<omega> (l, field_val)) = remove_only (stabilize \<omega>) (l, field_val)"
+            by (simp add: remove_only_stabilize)
+          then show "stabilize (remove_only \<omega> (l, field_val)) \<in> {remove_only \<omega> (l, field_val) |\<omega> l. \<omega> \<in> P \<and> semantify_addr r \<omega> = Some l}"
+            by (smt (verit, ccfv_threshold) AbstractSemantics.get_store_stabilize CollectI TypedEqui.self_framing_typedE TypedEqui.typed_state_axioms \<open>\<omega> \<in> P\<close> \<open>get_m \<omega> (l, field_val) = 1 \<and> semantify_addr r \<omega> = Some l\<close> asm0(3) asm1(2) semantify_addr_equiv typed_state.typed_assertionE)
+          show "TypedEqui.typed \<Delta> (remove_only \<omega> (l, field_val))"
+            by (meson TypedEqui.typed_assertion_def TypedEqui.typed_state_axioms \<open>\<omega> \<in> P\<close> asm0(3) calculation(1) greater_def typed_state.typed_smaller)
+        qed
+        ultimately show "\<omega> \<in> TypedEqui.Stabilize_typed \<Delta> (full_ownership r) \<otimes> ?F"
+          using commutative x_elem_set_product by fastforce
+      qed
+      show "TypedEqui.Stabilize_typed \<Delta> (full_ownership_with_val r e) \<otimes> ?F \<subseteq> Q \<otimes> atrue \<Delta>"
+      proof
+        fix \<omega>' assume "\<omega>' \<in> TypedEqui.Stabilize_typed \<Delta> (full_ownership_with_val r e) \<otimes> ?F"
+        then obtain ptr f where r: "Some \<omega>' = ptr \<oplus> f" "ptr \<in> TypedEqui.Stabilize_typed \<Delta> (full_ownership_with_val r e)" "f \<in> ?F"
+          by (meson x_elem_set_product)
+        then obtain l where "get_store (stabilize ptr) r = Some (VRef (Address l)) \<and> get_m (stabilize ptr) (l, field_val) = 1
+  \<and> get_h (stabilize ptr) (l, field_val) = Some (VInt (edenot e (get_store (stabilize ptr))))"
+          by (smt (verit, ccfv_SIG) CollectD ConcreteSemantics.stabilize_typed_elem full_ownership_with_val_def)
+        then have "get_store ptr r = Some (VRef (Address l)) \<and> get_m ptr (l, field_val) = 1
+  \<and> get_h ptr (l, field_val) = Some (VInt (edenot e (get_store ptr)))"
+          by (simp add: stabilize_value_persists)
+        then have "get_store \<omega>' r = Some (VRef (Address l)) \<and> get_m \<omega>' (l, field_val) = 1
+  \<and> get_h \<omega>' (l, field_val) = Some (VInt (edenot e (get_store \<omega>')))"
+          using r(1) greater_charact larger_mask_full
+          by (metis (no_types, lifting) in_set_sum is_in_set_sum r(3) read_helper singletonD state_add_iff)
+
+        moreover obtain \<omega> l' where "stabilize f = remove_only \<omega> (l', field_val)" "\<omega> \<in> P" "semantify_addr r \<omega> = Some l'"
+          by (smt (verit) CollectD ConcreteSemantics.stabilize_typed_elem r(3))
+        then have "l = l'"
+          by (metis (no_types, lifting) AbstractSemantics.get_store_stabilize \<open>get_store (stabilize ptr) r = Some (VRef (Address l)) \<and> get_m (stabilize ptr) (l, field_val) = 1 \<and> get_h (stabilize ptr) (l, field_val) = Some (VInt (edenot e (get_store (stabilize ptr))))\<close> full_add_defined get_address_simp get_store_set_state option.distinct(1) r(1) remove_only_def semantify_addr_equiv)
+
+        moreover have "\<omega>' \<succeq> update_heap_val \<omega> (l, field_val) (VInt (edenot e (get_store \<omega>')))"
+        proof (rule greater_equiI)
+          show "get_m \<omega>' \<succeq> get_m (update_heap_val \<omega> (l, field_val) (VInt (edenot e (get_store \<omega>'))))"
+          proof (rule greaterI)
+            fix la show "get_m \<omega>' la \<succeq> get_m (update_heap_val \<omega> (l, field_val) (VInt (edenot e (get_store \<omega>')))) la"
+              apply (cases "(l, field_val) = la")
+               apply (smt (verit) CollectD \<open>\<omega> \<in> P\<close> \<open>semantify_addr r \<omega> = Some l'\<close> asm1(3) calculation(1) calculation(2) entails_def get_state_set_state get_vh_vm_set_value(2) option.sel subsetD succ_refl)
+              by (smt (verit, ccfv_threshold) \<open>stabilize f = remove_only \<omega> (l', field_val)\<close> calculation(2) fun_plus_iff fun_upd_apply get_m_stabilize get_state_set_state get_vh_vm_set_value(2) get_vm_additive greater_equiv r(1) remove_only_charact(2) state_add_iff)
+          qed
+          show "get_h \<omega>' \<succeq> get_h (update_heap_val \<omega> (l, field_val) (VInt (edenot e (get_store \<omega>'))))"
+          proof (rule greaterI)
+            fix la show "get_h \<omega>' la \<succeq> get_h (update_heap_val \<omega> (l, field_val) (VInt (edenot e (get_store \<omega>')))) la"
+              apply (cases "(l, field_val) = la")
+              using calculation(1) succ_refl apply fastforce
+              apply (cases "get_h (update_heap_val \<omega> (l, field_val) (VInt (edenot e (get_store \<omega>')))) la")
+               apply (simp add: greater_equiv)
+              by (metis (no_types, opaque_lifting) \<open>stabilize f = remove_only \<omega> (l', field_val)\<close> calculation(2) fun_upd_other get_state_set_state get_vh_vm_set_value(1) greater_equiv greater_state_has_greater_parts(3) r(1) read_field.simps read_field_mono remove_only_charact(1) stabilize_value_persists succ_refl)
+          qed
+          show "get_store \<omega>' = get_store (update_heap_val \<omega> (l, field_val) (VInt (edenot e (get_store \<omega>'))))"
+            by (metis (no_types, lifting) AbstractSemantics.get_store_stabilize \<open>stabilize f = remove_only \<omega> (l', field_val)\<close> full_add_charact(1) full_add_defined get_store_set_state r(1) remove_only_def)
+          show "get_trace \<omega>' = get_trace (update_heap_val \<omega> (l, field_val) (VInt (edenot e (get_store \<omega>'))))"
+            by (metis \<open>stabilize f = remove_only \<omega> (l', field_val)\<close> get_trace_set_state get_trace_stabilize greater_equiv greater_state_has_greater_parts(2) r(1) remove_only_def)
+        qed
+        moreover have "update_heap_val \<omega> (l, field_val) (VInt (edenot e (get_store \<omega>'))) \<in> Q"
+          using \<open>l = l'\<close>
+          by (smt (verit, ccfv_SIG) AbstractSemantics.get_store_stabilize ConcreteSemantics.stabilize_typed_elem \<open>\<omega> \<in> P\<close> \<open>get_store ptr r = Some (VRef (Address l)) \<and> get_m ptr (l, field_val) = 1 \<and> get_h ptr (l, field_val) = Some (VInt (edenot e (get_store ptr)))\<close> \<open>semantify_addr r \<omega> = Some l'\<close> \<open>stabilize f = remove_only \<omega> (l', field_val)\<close> asm1(1) full_add_charact(1) full_add_defined get_store_set_state in_update_value r(1) r(2) remove_only_def semantify_exp_def snd_conv typed_get_vh)
+        ultimately show "\<omega>' \<in> Q \<otimes> atrue \<Delta>"
+          by (meson TypedEqui.typed_assertionE TypedEqui.typed_state_axioms \<open>\<omega>' \<in> TypedEqui.Stabilize_typed \<Delta> (full_ownership_with_val r e) \<otimes> TypedEqui.Stabilize_typed \<Delta> {remove_only \<omega> (l, field_val) |\<omega> l. \<omega> \<in> P \<and> semantify_addr r \<omega> = Some l}\<close> in_times_atrue typed_state.typed_Stabilize_typed typed_state.typed_star)
+      qed
+    qed
+  qed
+qed
+
+
+definition semantify_heap_loc :: "var \<Rightarrow> (int equi_state, int val) AbstractSemantics.exp" where
+  "semantify_heap_loc r \<omega> =
+  (if (\<exists>l v. get_store \<omega> r = Some (VRef (Address l)) \<and> get_h \<omega> (l, field_val) = Some (VInt v))
+  then Some (the (get_h \<omega> (SOME l. get_store \<omega> r = Some (VRef (Address l)), field_val)))
+  else None)"
+
+lemma convert_proof_read:
+  assumes "ConcreteSemantics.SL_proof \<Delta> P (LocalAssign x (semantify_heap_loc r)) Q"
+     (* and "custom_context \<Delta> = type_ctxt_heap" *)
+  shows "\<Delta> \<turnstile>CSL [P] Cread x r [Q]"
+  using assms(1)
+proof (rule ConcreteSemantics.SL_proof_LocalAssign_elim)
+  assume asm0: "Q = ConcreteSemantics.post_substitute_var_assert x (semantify_heap_loc r) P"
+    "framed_by_exp P (semantify_heap_loc r)"
+    "TypedEqui.self_framing_typed \<Delta> P" "TypedEqui.typed_assertion \<Delta> P"
+
+  have r: "\<And>\<omega>. \<omega> \<in> P \<Longrightarrow> (\<exists>l. get_store \<omega> r = Some (VRef (Address l)) \<and> get_m \<omega> (l, field_val) > 0
+  \<and> (\<exists>v. get_h \<omega> (l, field_val) = Some (VInt v)))"
+  proof -
+    fix \<omega>
+    assume "\<omega> \<in> P"
+    then obtain l v where "get_store \<omega> r = Some (VRef (Address l))" "get_h \<omega> (l, field_val) = Some (VInt v)"
+      by (metis asm0(2) framed_by_exp_def semantify_heap_loc_def)
+    moreover have "stabilize \<omega> \<in> P"
+      using TypedEqui.self_framing_typedE TypedEqui.typed_state_axioms \<open>\<omega> \<in> P\<close> asm0(3) asm0(4) typed_state.typed_assertionE by blast
+    then have "get_h (stabilize \<omega>) (l, field_val) = Some (VInt v)"
+      by (metis (no_types, lifting) AbstractSemantics.get_store_stabilize asm0(2) calculation(1) calculation(2) framed_by_exp_def get_address_simp semantify_heap_loc_def stabilize_value_persists)
+    then have "get_m \<omega> (l, field_val) > 0"
+      using EquiSemAuxLemma.gr_0_is_ppos stable_virtual_state_def by fastforce
+    then show "(\<exists>l. get_store \<omega> r = Some (VRef (Address l)) \<and> get_m \<omega> (l, field_val) > 0
+  \<and> (\<exists>v. get_h \<omega> (l, field_val) = Some (VInt v)))"
+      using calculation(1) calculation(2) by blast
+  qed
+
+  show "\<Delta> \<turnstile>CSL [P] Cread x r [Q]"
+  proof (rule RuleCons)
+    show "\<Delta> \<turnstile>CSL [P] Cread x r [read_result P x r]"
+    proof (rule RuleRead)
+      show "P \<subseteq> read_perm r" (* Should come from framed_by_exp *)
+        using r
+        unfolding read_perm_def by (simp add: subsetI)
+    qed
+    show "read_result P x r \<subseteq> Q"
+    proof
+      fix \<omega>' assume "\<omega>' \<in> read_result P x r"
+      then obtain \<omega> l where "\<omega>' = TypedEqui.assign_var_state x (get_h \<omega> (l, field_val)) \<omega>"
+          "\<omega> \<in> P" "get_store \<omega> r = Some (VRef (Address l))"
+        unfolding read_result_def by blast
+      moreover have "get_h \<omega> (l, field_val) = (if (\<exists>l v. get_store \<omega> r = Some (VRef (Address l)) \<and> get_h \<omega> (l, field_val) = Some (VInt v))
+            then Some (the (get_h \<omega> (SOME l. get_store \<omega> r = Some (VRef (Address l)), field_val))) else None)"
+        by (smt (verit, del_insts) calculation(2) calculation(3) get_address_simp option.distinct(1) option.expand option.sel r someI_ex vstate_wf_imp)
+      ultimately show "\<omega>' \<in> Q" using asm0(1)
+        unfolding ConcreteSemantics.post_substitute_var_assert_def ConcreteSemantics.substitute_var_state_def
+          semantify_heap_loc_def by force
+    qed
+  qed (simp)
+qed
+
+
+
 fun translate :: "cmd \<Rightarrow> (v_stmt \<times> v_stmt set)" where
   "translate Cskip = (Skip, {})"
+| "translate (Cassign x e) = (LocalAssign x (semantify_exp e), {})"
+
 | "translate (Calloc r e) = ((Havoc r;; Inhale (full_ownership_with_val r e)), {})"
+| "translate (Cfree r) = (Exhale (Stabilize (full_ownership r)), {})"
+| "translate (Cwrite r e) = (Custom (FieldAssign (semantify_addr r) field_val (semantify_exp e)), {})"
+| "translate (Cread x r) = (LocalAssign x (semantify_heap_loc r), {})"
+
+| "translate (Cseq C1 C2) = (let r1 = translate C1 in let r2 = translate C2 in
+  (fst r1;; fst r2, snd r1 \<union> snd r2))"
+
+| "translate (Cif b C1 C2) = (If (semantify_bexp b) (fst (translate C1)) (fst (translate C2)), snd (translate C1) \<union> snd (translate C2))"
+
+
 | "translate ({P1} C1 {Q1} || {P2} C2 {Q2}) =
   ((Exhale (P1 \<otimes> P2);; ConcreteSemantics.havoc_list (wrL C1 @ wrL C2);; Inhale (Q1 \<otimes> Q2)),
   let r1 = translate C1 in let r2 = translate C2 in
   { (Inhale P1;; fst r1;; Exhale Q1), (Inhale P2;; fst r2;; Exhale Q2) } \<union> snd r1 \<union> snd r2)"
 
-thm ConcreteSemantics.Viper_implies_SL_proof
-thm emp_star_right_id
+lemma CSL_weaken_post_atrue:
+  assumes "\<Delta> \<turnstile>CSL [P] C [Q]"
+      and "TypedEqui.typed_assertion \<Delta> Q"
+  shows "\<Delta> \<turnstile>CSL [P] C [Q \<otimes> atrue \<Delta>]"
+  using assms(1)
+proof (rule RuleCons)
+  show "Q \<subseteq> Q \<otimes> atrue \<Delta>"
+    using add_set_commm assms(2) conjunct_with_true_entails by blast
+qed (simp)
 
-definition has_Viper_proof where
-  "has_Viper_proof \<Delta> Cv \<longleftrightarrow> (\<exists>B. ConcreteSemantics.SL_proof \<Delta> emp Cv B)"
-
-definition translation_has_proof where
-  "translation_has_proof \<Delta> P C Q \<longleftrightarrow> (\<exists>B. ConcreteSemantics.SL_proof \<Delta> P (fst (translate C)) (B \<otimes> Q)) \<and>
-  (\<forall>Cv \<in> snd (translate C). has_Viper_proof \<Delta> Cv)"
-
-lemma translation_has_proofI:
-  assumes "\<exists>B. ConcreteSemantics.SL_proof \<Delta> P (fst (translate C)) (B \<otimes> Q)"
-      and "\<And>Cv. Cv \<in> snd (translate C) \<Longrightarrow> has_Viper_proof \<Delta> Cv"
-    shows "translation_has_proof \<Delta> P C Q"
-  by (simp add: assms(1) assms(2) translation_has_proof_def)
+lemma CSL_add_atrue:
+  assumes "\<Delta> \<turnstile>CSL [P] C [Q]"
+      and "TypedEqui.self_framing_typed \<Delta> P"
+      and "TypedEqui.typed_assertion \<Delta> P"
+    shows "\<Delta> \<turnstile>CSL [P \<otimes> atrue \<Delta>] C [Q \<otimes> atrue \<Delta>]"
+  by (rule RuleFrame) (simp_all add: assms)
 
 
-lemma has_proof_with_inhale_exhale:
-  assumes "has_Viper_proof \<Delta> (Inhale P;; C;; Exhale Q)"
-  shows "\<exists>R B. ConcreteSemantics.SL_proof \<Delta> P C R \<and> entails R (B \<otimes> Q)"
-proof -
-  obtain B where "ConcreteSemantics.SL_proof \<Delta> emp ((Inhale P;; C);; Exhale Q) B"
-    using assms has_Viper_proof_def by blast
-  then show ?thesis
-  proof (rule ConcreteSemantics.SL_proof_Seq_elim)
-    fix R1 assume asm0: "ConcreteSemantics.SL_proof \<Delta> emp (abs_stmt.Inhale P ;; C) R1"
-      "ConcreteSemantics.SL_proof \<Delta> R1 (abs_stmt.Exhale Q) B"
-    then have "entails R1 (B \<otimes> Q)" by auto (* ConcreteSemantics.SL_proof_Exhale_elim[OF asm0(2)] *)
-    show "\<exists>R B. ConcreteSemantics.SL_proof \<Delta> P C R \<and> entails R (B \<otimes> Q)"
-    proof (rule ConcreteSemantics.SL_proof_Seq_elim[OF asm0(1)])
-      fix R0 assume asm1: "ConcreteSemantics.SL_proof \<Delta> emp (abs_stmt.Inhale P) R0"
-        "ConcreteSemantics.SL_proof \<Delta> R0 C R1"
-      then have "ConcreteSemantics.SL_proof \<Delta> P C R1"
-        by auto
-      then show "\<exists>R B. ConcreteSemantics.SL_proof \<Delta> P C R \<and> entails R (B \<otimes> Q)"
-        using \<open>entails R1 (B \<otimes> Q)\<close> by blast
+definition proof_obligations_valid where
+  "proof_obligations_valid \<Delta> S \<longleftrightarrow> (\<forall>Cv \<in> S. \<exists>B. ConcreteSemantics.SL_proof \<Delta> (atrue \<Delta>) Cv B)"
+
+lemma proof_obligations_valid_union:
+  "proof_obligations_valid \<Delta> (S1 \<union> S2) \<longleftrightarrow> proof_obligations_valid \<Delta> S1 \<and> proof_obligations_valid \<Delta> S2"
+  by (meson Un_iff proof_obligations_valid_def)
+
+definition invariant_translate where
+  "invariant_translate \<Delta> P C Q \<longleftrightarrow>
+  ((proof_obligations_valid \<Delta> (snd (translate C)) \<and> ConcreteSemantics.SL_proof \<Delta> P (fst (translate C)) Q) \<longrightarrow> \<Delta> \<turnstile>CSL [P \<otimes> atrue \<Delta>] C [Q \<otimes> atrue \<Delta>])"
+
+lemma invariant_translateE:
+  assumes "invariant_translate \<Delta> P C Q"
+      and "proof_obligations_valid \<Delta> (snd (translate C))"
+      and "ConcreteSemantics.SL_proof \<Delta> P (fst (translate C)) Q"
+    shows "\<Delta> \<turnstile>CSL [P \<otimes> atrue \<Delta>] C [Q \<otimes> atrue \<Delta>]"
+  using assms(1) assms(2) assms(3) invariant_translate_def by blast
+
+
+lemma invariant_translateI:
+  assumes "proof_obligations_valid \<Delta> (snd (translate C)) \<Longrightarrow> ConcreteSemantics.SL_proof \<Delta> P (fst (translate C)) Q
+    \<Longrightarrow> \<Delta> \<turnstile>CSL [P \<otimes> atrue \<Delta>] C [Q \<otimes> atrue \<Delta>]"
+  shows "invariant_translate \<Delta> P C Q"
+  using assms invariant_translate_def proof_obligations_valid_def by blast
+
+lemma invariant_translate_simpler:
+  assumes "ConcreteSemantics.SL_proof \<Delta> P (fst (translate C)) Q \<Longrightarrow> \<Delta> \<turnstile>CSL [P] C [Q]"
+  shows "invariant_translate \<Delta> P C Q"
+  by (meson CSL_add_atrue ConcreteSemantics.semantics_axioms assms invariant_translateI semantics.proof_then_self_framing semantics.proof_then_typed)
+
+corollary invariant_translate_skip:
+  "invariant_translate \<Delta> P Cskip Q"
+  using convert_proof_skip invariant_translate_simpler by fastforce
+
+corollary invariant_translate_assign:
+  "invariant_translate \<Delta> P (Cassign x e) Q"
+  using convert_proof_assign invariant_translate_simpler by fastforce
+
+corollary invariant_translate_alloc:
+  assumes "well_typed_cmd \<Delta> (Calloc r e)"
+      and "wf_stmt \<Delta> (Calloc r e)"
+    shows "invariant_translate \<Delta> P (Calloc r e) Q"
+  using assms(1) assms(2) cmd.distinct(37) convert_proof_alloc invariant_translate_simpler by fastforce
+
+lemma atrue_twice_same:
+  "atrue \<Delta> \<otimes> atrue \<Delta> \<subseteq> atrue \<Delta>"
+  unfolding atrue_def add_set_def
+  by (smt (z3) Collect_mono_iff TypedEqui.typed_sum mem_Collect_eq)
+
+lemma atrue_twice_equal:
+  "atrue \<Delta> \<otimes> atrue \<Delta> = atrue \<Delta>"
+proof
+  show "atrue \<Delta> \<subseteq> atrue \<Delta> \<otimes> atrue \<Delta>"
+  proof
+    fix x assume "x \<in> atrue \<Delta>"
+    then have "Some x = x \<oplus> |x|"
+      using core_is_smaller by blast
+    then have "|x| \<in> atrue \<Delta>"
+      using TypedEqui.typed_core \<open>x \<in> atrue \<Delta>\<close> atrue_def by blast
+    then show "x \<in> atrue \<Delta> \<otimes> atrue \<Delta>"
+      using \<open>Some x = x \<oplus> |x|\<close> \<open>x \<in> atrue \<Delta>\<close> x_elem_set_product by blast
+  qed
+qed (simp add: atrue_twice_same)
+
+
+corollary invariant_translate_free:
+  "invariant_translate \<Delta> P (Cfree r) Q"
+proof (rule invariant_translateI)
+  assume asm0: "ConcreteSemantics.SL_proof \<Delta> P (fst (translate (Cfree r))) Q"
+  then have "\<Delta> \<turnstile>CSL [P \<otimes> atrue \<Delta>] Cfree r [(Q \<otimes> atrue \<Delta>) \<otimes> atrue \<Delta>]"
+    using RuleFrame[OF convert_proof_free]
+    by (simp add: ConcreteSemantics.proof_then_self_framing ConcreteSemantics.proof_then_typed)
+  then show "\<Delta> \<turnstile>CSL [P \<otimes> atrue \<Delta>] Cfree r [Q \<otimes> atrue \<Delta>]"
+    by (simp add: add_set_asso atrue_twice_equal)
+qed
+
+corollary invariant_translate_write:
+  "invariant_translate \<Delta> P (Cwrite r e) Q"
+proof (rule invariant_translateI)
+  assume asm0: "ConcreteSemantics.SL_proof \<Delta> P (fst (translate (Cwrite r e))) Q"
+  then have "\<Delta> \<turnstile>CSL [P \<otimes> atrue \<Delta>] Cwrite r e [(Q \<otimes> atrue \<Delta>) \<otimes> atrue \<Delta>]"
+    using RuleFrame[OF convert_proof_write]
+    by (simp add: ConcreteSemantics.proof_then_self_framing ConcreteSemantics.proof_then_typed)
+  then show "\<Delta> \<turnstile>CSL [P \<otimes> atrue \<Delta>] Cwrite r e [Q \<otimes> atrue \<Delta>]"
+    by (simp add: add_set_asso atrue_twice_equal)
+qed
+
+corollary invariant_translate_read:
+  "invariant_translate \<Delta> P (Cread x r) Q"
+  using convert_proof_read invariant_translate_simpler by fastforce
+
+
+lemma invariant_translate_seq:
+  assumes "\<And>R. invariant_translate \<Delta> P C1 R"
+      and "\<And>R. invariant_translate \<Delta> R C2 Q"
+    shows "invariant_translate \<Delta> P (Cseq C1 C2) Q"
+proof (rule invariant_translateI)
+  assume asm0: "proof_obligations_valid \<Delta> (snd (translate (Cseq C1 C2)))"
+    "ConcreteSemantics.SL_proof \<Delta> P (fst (translate (Cseq C1 C2))) Q"
+  then obtain R where r: "ConcreteSemantics.SL_proof \<Delta> P (fst (translate C1)) R"
+      "ConcreteSemantics.SL_proof \<Delta> R (fst (translate C2)) Q"
+    by (metis ConcreteSemantics.SL_proof_Seq_elim fst_eqD translate.simps(7))
+  show "\<Delta> \<turnstile>CSL [P \<otimes> atrue \<Delta>] Cseq C1 C2 [Q \<otimes> atrue \<Delta>]"
+  proof (rule RuleSeq)
+    show "\<Delta> \<turnstile>CSL [P \<otimes> atrue \<Delta>] C1 [R \<otimes> atrue \<Delta>]"
+      using assms(1)[of R] r
+      unfolding invariant_translate_def
+      by (metis asm0(1) proof_obligations_valid_union snd_conv translate.simps(7))
+    show "\<Delta> \<turnstile>CSL [R \<otimes> atrue \<Delta>] C2 [Q \<otimes> atrue \<Delta>]"
+    proof (rule RuleCons)
+      show "\<Delta> \<turnstile>CSL [R \<otimes> atrue \<Delta>] C2 [(Q \<otimes> atrue \<Delta>) \<otimes> atrue \<Delta>]"
+          using assms(2)[of R] asm0
+          unfolding invariant_translate_def proof_obligations_valid_def
+          by (metis (no_types, lifting) Un_iff add_set_asso atrue_twice_equal r(2) snd_conv translate.simps(7))
+      show "Q \<otimes> atrue \<Delta> \<otimes> atrue \<Delta> \<subseteq> Q \<otimes> atrue \<Delta>"
+        by (simp add: add_set_asso add_set_mono atrue_twice_same)
+    qed (simp)
+  qed
+qed
+
+
+lemma invariant_translate_inhale_exhale_get_proof:
+  assumes "\<And>P Q. invariant_translate \<Delta> P C Q"
+      and "ConcreteSemantics.SL_proof \<Delta> P (Inhale A;; fst (translate C);; Exhale B) Q"
+      and "proof_obligations_valid \<Delta> (snd (translate C))"
+    shows "\<Delta> \<turnstile>CSL [P \<otimes> A \<otimes> atrue \<Delta>] C [Q \<otimes> B \<otimes> atrue \<Delta>]"
+  using assms(2)
+proof (rule ConcreteSemantics.SL_proof_Seq_elim)
+  fix R1 assume asm0: "ConcreteSemantics.SL_proof \<Delta> P (abs_stmt.Inhale A ;; fst (translate C)) R1"
+    "ConcreteSemantics.SL_proof \<Delta> R1 (abs_stmt.Exhale B) Q"
+  then have "entails R1 (Q \<otimes> B)" by auto
+  show "\<Delta> \<turnstile>CSL [P \<otimes> A \<otimes> atrue \<Delta>] C [Q \<otimes> B \<otimes> atrue \<Delta>]"
+  proof (rule ConcreteSemantics.SL_proof_Seq_elim[OF asm0(1)])
+    fix R0 assume asm1: "ConcreteSemantics.SL_proof \<Delta> P (abs_stmt.Inhale A) R0"
+          "ConcreteSemantics.SL_proof \<Delta> R0 (fst (translate C)) R1"
+    then have "ConcreteSemantics.SL_proof \<Delta> (P \<otimes> A) (fst (translate C)) R1"
+      by auto
+    show "\<Delta> \<turnstile>CSL [P \<otimes> A \<otimes> atrue \<Delta>] C [Q \<otimes> B \<otimes> atrue \<Delta>]"
+    proof (rule RuleCons)
+      show "\<Delta> \<turnstile>CSL [P \<otimes> A \<otimes> atrue \<Delta>] C [R1 \<otimes> atrue \<Delta>]"
+        using \<open>ConcreteSemantics.SL_proof \<Delta> (P \<otimes> A) (fst (translate C)) R1\<close> assms(1) assms(3) invariant_translate_def by blast
+      show "R1 \<otimes> atrue \<Delta> \<subseteq> Q \<otimes> B \<otimes> atrue \<Delta>"
+        by (meson \<open>entails R1 (Q \<otimes> B)\<close> add_set_mono entails_def order_refl)
+    qed (simp)
+  qed
+qed
+
+
+lemma drop_conjunct_entails:
+  assumes "TypedEqui.typed_assertion \<Delta> A"
+  shows "A \<otimes> B \<otimes> atrue \<Delta> \<subseteq> B \<otimes> atrue \<Delta>"
+  by (smt (verit) TypedEqui.typed_assertion_def add_set_asso add_set_commm add_set_def assms atrue_def atrue_twice_equal mem_Collect_eq subsetI)
+
+
+(*
+| "translate ({P1} C1 {Q1} || {P2} C2 {Q2}) =
+  ((Exhale (P1 \<otimes> P2);; ConcreteSemantics.havoc_list (wrL C1 @ wrL C2);; Inhale (Q1 \<otimes> Q2)),
+  let r1 = translate C1 in let r2 = translate C2 in
+  { (Inhale P1;; fst r1;; Exhale Q1), (Inhale P2;; fst r2;; Exhale Q2) } \<union> snd r1 \<union> snd r2)"
+*)
+
+
+lemma typed_self_framing_star:
+  assumes "TypedEqui.self_framing_typed \<Delta> A"
+      and "TypedEqui.self_framing_typed \<Delta> B"
+    shows "TypedEqui.self_framing_typed \<Delta> (A \<otimes> B)"
+proof (rule TypedEqui.self_framing_typedI)
+  fix \<omega> assume asm0: "TypedEqui.typed \<Delta> \<omega>"
+  show "(\<omega> \<in> A \<otimes> B) = (stabilize \<omega> \<in> A \<otimes> B)"
+  proof
+    assume "\<omega> \<in> A \<otimes> B"
+    then obtain a b where "Some \<omega> = a \<oplus> b" "a \<in> A" "b \<in> B"
+      by (meson x_elem_set_product)
+    then show "stabilize \<omega> \<in> A \<otimes> B"
+      by (metis (no_types, lifting) TypedEqui.typed_state_axioms asm0 assms(1) assms(2) greater_def greater_equiv stabilize_sum typed_state.self_framing_typedE typed_state.typed_smaller x_elem_set_product)
+  next
+    assume "stabilize \<omega> \<in> A \<otimes> B"
+    then obtain a b where "Some (stabilize \<omega>) = a \<oplus> b" "a \<in> A" "b \<in> B"
+      by (meson x_elem_set_product)
+    then obtain b' where "Some b' = b \<oplus> |\<omega>|"
+      by (metis (no_types, opaque_lifting) asso2 decompose_stabilize_pure option.exhaust_sel)
+    then have "stabilize b' = stabilize b"
+      using plus_pure_stabilize_eq by blast
+    moreover have "TypedEqui.typed \<Delta> b'"
+      by (smt (verit, ccfv_SIG) TypedEqui.typed_state_axioms \<open>Some (stabilize \<omega>) = a \<oplus> b\<close> \<open>Some b' = b \<oplus> |\<omega>|\<close> addition_bigger asm0 commutative decompose_stabilize_pure greater_def typed_state.typed_smaller)
+    ultimately have "b' \<in> B"
+      by (metis (no_types, lifting) TypedEqui.typed_smaller TypedEqui.typed_state_axioms \<open>Some b' = b \<oplus> |\<omega>|\<close> \<open>b \<in> B\<close> assms(2) commutative greater_equiv typed_state.self_framing_typed_def)
+    then show "\<omega> \<in> A \<otimes> B"
+      by (metis (no_types, lifting) \<open>Some (stabilize \<omega>) = a \<oplus> b\<close> \<open>Some b' = b \<oplus> |\<omega>|\<close> \<open>a \<in> A\<close> asso1 decompose_stabilize_pure x_elem_set_product)
+  qed
+qed
+
+
+
+lemma self_framing_typed_star_atrue:
+  assumes "TypedEqui.self_framing_typed \<Delta> P"
+  shows "TypedEqui.self_framing_typed \<Delta> (P \<otimes> atrue \<Delta>)"
+  by (simp add: assms typed_self_framing_star)
+
+lemma typed_assertion_star_atrue:
+  assumes "TypedEqui.typed_assertion \<Delta> P"
+  shows "TypedEqui.typed_assertion \<Delta> (P \<otimes> atrue \<Delta>)"
+  by (simp add: TypedEqui.typed_star assms)
+
+
+
+
+lemma invariant_translate_parallel:
+  assumes "\<And>P Q. invariant_translate \<Delta> P C1 Q"
+      and "\<And>P Q. invariant_translate \<Delta> P C2 Q"
+      and "ConcreteSemantics.wf_abs_stmt \<Delta> (ConcreteSemantics.havoc_list (wrL C1 @ wrL C2))"
+      and "wf_stmt \<Delta> ({P1} C1 {Q1} || {P2} C2 {Q2})"
+    shows "invariant_translate \<Delta> P ({P1} C1 {Q1} || {P2} C2 {Q2}) Q"
+proof (rule invariant_translateI)
+  assume asm0: "proof_obligations_valid \<Delta> (snd (translate {P1} C1 {Q1} || {P2} C2 {Q2}))"
+    "ConcreteSemantics.SL_proof \<Delta> P (fst (translate {P1} C1 {Q1} || {P2} C2 {Q2})) Q"
+  then have r0: "proof_obligations_valid \<Delta> (snd (translate C1)) \<and> proof_obligations_valid \<Delta> (snd (translate C2))"
+    using proof_obligations_valid_union
+    unfolding translate.simps by (metis sndI)
+  moreover obtain B1 where B1_def: "ConcreteSemantics.SL_proof \<Delta> (atrue \<Delta>) (Inhale P1;; fst (translate C1);; Exhale Q1) B1"
+    using asm0 unfolding translate.simps proof_obligations_valid_def
+    by (metis Un_iff insertCI snd_eqD)
+  moreover obtain B2 where B2_def: "ConcreteSemantics.SL_proof \<Delta> (atrue \<Delta>) (Inhale P2;; fst (translate C2);; Exhale Q2) B2"
+    using asm0 unfolding translate.simps proof_obligations_valid_def
+    by (metis Un_iff insertCI snd_eqD)
+  moreover have main: "ConcreteSemantics.SL_proof \<Delta> P (Exhale (P1 \<otimes> P2);; ConcreteSemantics.havoc_list (wrL C1 @ wrL C2);; Inhale (Q1 \<otimes> Q2)) Q"
+    using asm0 by simp
+  then obtain R0 R1 where R_defs:
+    "ConcreteSemantics.SL_proof \<Delta> P (abs_stmt.Exhale (P1 \<otimes> P2)) R0"
+    "ConcreteSemantics.SL_proof \<Delta> R0 (ConcreteSemantics.havoc_list (wrL C1 @ wrL C2)) R1"
+    "ConcreteSemantics.SL_proof \<Delta> R1 (abs_stmt.Inhale (Q1 \<otimes> Q2)) Q"
+    by (meson ConcreteSemantics.SL_proof_Seq_elim)
+  then have P_Q_R_rels:
+    "entails P (R0 \<otimes> (P1 \<otimes> P2)) \<and> Q = R1 \<otimes> (Q1 \<otimes> Q2)" by auto
+  moreover have "entails R0 R1 \<and> fvA \<Delta> R1 \<subseteq> fvA \<Delta> R0 - (set (wrL C1 @ wrL C2))"
+    using ConcreteSemantics.SL_proof_Havoc_list_elim R_defs(2) assms(3) by blast
+(* R1 is the frame! *)
+
+  show "\<Delta> \<turnstile>CSL [P \<otimes> atrue \<Delta>] {P1} C1 {Q1} || {P2} C2 {Q2} [Q \<otimes> atrue \<Delta>]"
+  proof (rule RuleCons)
+    show "\<Delta> \<turnstile>CSL [((P1 \<otimes> atrue \<Delta>) \<otimes> (P2 \<otimes> atrue \<Delta>)) \<otimes> R1] {P1} C1 {Q1} || {P2} C2 {Q2} [((Q1 \<otimes> atrue \<Delta>) \<otimes> (Q2 \<otimes> atrue \<Delta>)) \<otimes> R1]"
+    proof (rule RuleFrame)
+      show "\<Delta> \<turnstile>CSL [P1 \<otimes> atrue \<Delta> \<otimes> (P2 \<otimes> atrue \<Delta>)] {P1} C1 {Q1} || {P2} C2 {Q2} [Q1 \<otimes> atrue \<Delta> \<otimes> (Q2 \<otimes> atrue \<Delta>)]"
+      proof (rule RulePar)
+        show "\<Delta> \<turnstile>CSL [P1 \<otimes> atrue \<Delta>] C1 [Q1 \<otimes> atrue \<Delta>]"
+        proof (rule RuleCons)
+          show "\<Delta> \<turnstile>CSL [atrue \<Delta> \<otimes> P1 \<otimes> atrue \<Delta>] C1 [B1 \<otimes> Q1 \<otimes> atrue \<Delta>]"
+            using invariant_translate_inhale_exhale_get_proof[OF assms(1) B1_def]
+            using r0 by blast
+          show "B1 \<otimes> Q1 \<otimes> atrue \<Delta> \<subseteq> Q1 \<otimes> atrue \<Delta>"
+            using B1_def drop_conjunct_entails by blast
+          show "P1 \<otimes> atrue \<Delta> \<subseteq> atrue \<Delta> \<otimes> P1 \<otimes> atrue \<Delta>"
+            by (simp add: add_set_asso add_set_left_comm atrue_twice_equal)
+        qed
+        show "\<Delta> \<turnstile>CSL [P2 \<otimes> atrue \<Delta>] C2 [Q2 \<otimes> atrue \<Delta>]"
+        proof (rule RuleCons)
+          show "\<Delta> \<turnstile>CSL [atrue \<Delta> \<otimes> P2 \<otimes> atrue \<Delta>] C2 [B2 \<otimes> Q2 \<otimes> atrue \<Delta>]"
+            using invariant_translate_inhale_exhale_get_proof[OF assms(2) B2_def]
+            using r0 by blast
+          show "B2 \<otimes> Q2 \<otimes> atrue \<Delta> \<subseteq> Q2 \<otimes> atrue \<Delta>"
+            using B2_def drop_conjunct_entails by blast
+          show "P2 \<otimes> atrue \<Delta> \<subseteq> atrue \<Delta> \<otimes> P2 \<otimes> atrue \<Delta>"
+            by (simp add: add_set_asso add_set_left_comm atrue_twice_equal)
+        qed
+        show "disjoint (fvC C1 \<union> fvA \<Delta> (Q1 \<otimes> atrue \<Delta>)) (wrC C2)"
+          using assms(4) by auto
+        show "disjoint (fvC C2 \<union> fvA \<Delta> (Q2 \<otimes> atrue \<Delta>)) (wrC C1)"
+          using assms(4) by auto
+        show "TypedEqui.self_framing_typed \<Delta> (P1 \<otimes> atrue \<Delta>)"
+          using assms(4) self_framing_typed_star_atrue wf_stmt.simps(3) by blast
+        show "TypedEqui.self_framing_typed \<Delta> (P2 \<otimes> atrue \<Delta>)"
+          using assms(4) self_framing_typed_star_atrue by auto
+        show "TypedEqui.typed_assertion \<Delta> (P1 \<otimes> atrue \<Delta>)"
+          using assms(4) typed_assertion_star_atrue by auto
+        show "TypedEqui.typed_assertion \<Delta> (P2 \<otimes> atrue \<Delta>)"
+          using assms(4) typed_assertion_star_atrue by auto
+      qed
+      show "disjoint (fvA \<Delta> R1) (wrC {P1} C1 {Q1} || {P2} C2 {Q2})"
+        by (metis (mono_tags, opaque_lifting) Diff_subset_conv Orderings.order_eq_iff \<open>entails R0 R1 \<and> fvA \<Delta> R1 \<subseteq> fvA \<Delta> R0 - set (wrL C1 @ wrL C2)\<close> bot.extremum disjoint_minus disjoint_simps(2) disjoint_simps(3) sup.order_iff wrC.simps(7) wrC.simps(8) wrL.simps(7) wrL_wrC_same)
+      show "TypedEqui.self_framing_typed \<Delta> (P1 \<otimes> atrue \<Delta> \<otimes> (P2 \<otimes> atrue \<Delta>))"
+        by (meson assms(4) self_framing_typed_star_atrue typed_self_framing_star wf_stmt.simps(3))
+      show "TypedEqui.typed_assertion \<Delta> (P1 \<otimes> atrue \<Delta> \<otimes> (P2 \<otimes> atrue \<Delta>))"
+        using TypedEqui.typed_star assms(4) typed_assertion_star_atrue wf_stmt.simps(3) by blast
+      show "TypedEqui.self_framing_typed \<Delta> R1"
+        using R_defs(3) by blast
+      show "TypedEqui.typed_assertion \<Delta> R1"
+        using R_defs(3) by force
+    qed
+    show "P \<otimes> atrue \<Delta> \<subseteq> P1 \<otimes> atrue \<Delta> \<otimes> (P2 \<otimes> atrue \<Delta>) \<otimes> R1"
+    proof -
+      have "P \<otimes> atrue \<Delta> \<subseteq> (R0 \<otimes> (P1 \<otimes> P2)) \<otimes> atrue \<Delta>"
+        by (metis P_Q_R_rels add_set_mono atrue_twice_equal atrue_twice_same entails_def)
+      also have "... \<subseteq> R1 \<otimes> ((P1 \<otimes> P2) \<otimes> atrue \<Delta>)"
+        using \<open>entails R0 R1 \<and> fvA \<Delta> R1 \<subseteq> fvA \<Delta> R0 - set (wrL C1 @ wrL C2)\<close> add_set_asso add_set_mono entails_def by blast
+      also have "... \<subseteq> P1 \<otimes> atrue \<Delta> \<otimes> (P2 \<otimes> atrue \<Delta>) \<otimes> R1"
+        by (simp add: add_set_commm add_set_left_comm atrue_twice_equal)
+      finally show ?thesis by simp
+    qed
+    show "Q1 \<otimes> atrue \<Delta> \<otimes> (Q2 \<otimes> atrue \<Delta>) \<otimes> R1 \<subseteq> Q \<otimes> atrue \<Delta>"
+      by (simp add: P_Q_R_rels add_set_commm add_set_left_comm atrue_twice_equal)
+  qed
+qed
+
+(*
+Maybe prove? Need to prove that assertions are wf...
+lemma translation_wf:
+  assumes "wf_stmt \<Delta> C"
+      and "well_typed_cmd \<Delta> C"
+    shows "ConcreteSemantics.wf_abs_stmt \<Delta> (fst (translate C))"
+  using assms
+proof (induct C)
+  case (Cseq C1 C2)
+  then show ?case
+    by (metis ConcreteSemantics.wf_abs_stmt.simps(7) fst_eqD translate.simps(7) well_typed_cmd_aux.simps(2) wf_stmt.simps(1))
+next
+  ...
+qed (simp_all)
+*)
+
+lemma invariant_translate_if:
+  assumes "\<And>P Q. invariant_translate \<Delta> P C1 Q"
+      and "\<And>P Q. invariant_translate \<Delta> P C2 Q"
+    shows "invariant_translate \<Delta> P (Cif b C1 C2) Q"
+proof (rule invariant_translateI)
+  assume asm0: "proof_obligations_valid \<Delta> (snd (translate (Cif b C1 C2)))"
+    "ConcreteSemantics.SL_proof \<Delta> P (fst (translate (Cif b C1 C2))) Q"
+
+  show "\<Delta> \<turnstile>CSL [P \<otimes> atrue \<Delta>] Cif b C1 C2 [Q \<otimes> atrue \<Delta>]"
+  proof (rule ConcreteSemantics.SL_proof_If_elim)
+    show "ConcreteSemantics.SL_proof \<Delta> P (abs_stmt.If (semantify_bexp b) (fst (translate C1)) (fst (translate C2))) Q"
+      by (metis asm0(2) fst_eqD translate.simps(8))
+    fix B1 B2 assume asm1: "Q = B1 \<union> B2" "framed_by_exp P (semantify_bexp b)"
+       "ConcreteSemantics.SL_proof \<Delta> (P \<otimes> ConcreteSemantics.pure_typed \<Delta> (semantify_bexp b)) (fst (translate C1)) B1"
+       "ConcreteSemantics.SL_proof \<Delta> (P \<otimes> ConcreteSemantics.pure_typed \<Delta> (negate (semantify_bexp b))) (fst (translate C2)) B2"
+       "TypedEqui.self_framing_typed \<Delta> P" "TypedEqui.typed_assertion \<Delta> P"
+    show "\<Delta> \<turnstile>CSL [P \<otimes> atrue \<Delta>] Cif b C1 C2 [Q \<otimes> atrue \<Delta>]"
+    proof (rule RuleIf)
+      show "\<Delta> \<turnstile>CSL [(P \<otimes> atrue \<Delta>) \<inter> assertify_bexp b] C1 [Q \<otimes> atrue \<Delta>]"
+      proof (rule RuleCons)
+        show "\<Delta> \<turnstile>CSL [(P \<otimes> ConcreteSemantics.pure_typed \<Delta> (semantify_bexp b)) \<otimes> atrue \<Delta>] C1 [B1 \<otimes> atrue \<Delta>]"
+          by (metis asm0(1) asm1(3) assms(1) invariant_translateE proof_obligations_valid_union snd_conv translate.simps(8))
+        show "B1 \<otimes> atrue \<Delta> \<subseteq> Q \<otimes> atrue \<Delta>"
+          by (simp add: add_set_mono asm1(1))
+        show "(P \<otimes> atrue \<Delta>) \<inter> assertify_bexp b \<subseteq> (P \<otimes> ConcreteSemantics.pure_typed \<Delta> (semantify_bexp b)) \<otimes> atrue \<Delta>"
+        proof
+          fix \<omega> assume "\<omega> \<in> (P \<otimes> atrue \<Delta>) \<inter> assertify_bexp b"
+          then obtain p r where "Some \<omega> = p \<oplus> r" "p \<in> P" "bdenot b (get_store \<omega>)"
+            using in_set_sum[of \<omega> P "atrue \<Delta>"] assertify_bexp_def
+            by (smt (verit) Int_iff commutative greater_equiv mem_Collect_eq)
+          then have "|p| \<in> ConcreteSemantics.pure_typed \<Delta> (semantify_bexp b)"
+            unfolding ConcreteSemantics.pure_typed_def semantify_bexp_def
+            by (smt (verit, ccfv_SIG) ConcreteSemantics.get_store_Ag_simplifies TypedEqui.typed_assertionE TypedEqui.typed_core asm1(6) full_add_charact(1) full_core_def max_projection_prop_pure_core mem_Collect_eq mpp_prop)
+          then have "p \<in> P \<otimes> ConcreteSemantics.pure_typed \<Delta> (semantify_bexp b)"
+            using \<open>p \<in> P\<close> core_is_smaller x_elem_set_product by blast
+          then show "\<omega> \<in> (P \<otimes> ConcreteSemantics.pure_typed \<Delta> (semantify_bexp b)) \<otimes> atrue \<Delta>"
+            using TypedEqui.typed_state_axioms \<open>Some \<omega> = p \<oplus> r\<close> \<open>\<omega> \<in> (P \<otimes> atrue \<Delta>) \<inter> assertify_bexp b\<close> asm1(6) greater_def in_times_atrue typed_assertion_star_atrue typed_state.typed_assertionE by blast
+        qed
+      qed
+
+      show "\<Delta> \<turnstile>CSL [(P \<otimes> atrue \<Delta>) \<inter> assertify_bexp (Bnot b)] C2 [Q \<otimes> atrue \<Delta>]"
+      proof (rule RuleCons)
+        show "\<Delta> \<turnstile>CSL [(P \<otimes> ConcreteSemantics.pure_typed \<Delta> (negate (semantify_bexp b))) \<otimes> atrue \<Delta>] C2 [B2 \<otimes> atrue \<Delta>]"
+          by (metis asm0(1) asm1(4) assms(2) invariant_translateE proof_obligations_valid_union snd_conv translate.simps(8))
+        show "B2 \<otimes> atrue \<Delta> \<subseteq> Q \<otimes> atrue \<Delta>"
+          by (simp add: add_set_mono asm1(1))
+        show "(P \<otimes> atrue \<Delta>) \<inter> assertify_bexp (Bnot b) \<subseteq> P \<otimes> ConcreteSemantics.pure_typed \<Delta> (negate (semantify_bexp b)) \<otimes> atrue \<Delta>"
+        proof
+          fix \<omega> assume "\<omega> \<in> (P \<otimes> atrue \<Delta>) \<inter> assertify_bexp (Bnot b)"
+          then obtain p r where "Some \<omega> = p \<oplus> r" "p \<in> P" "bdenot (Bnot b) (get_store \<omega>)"
+            using in_set_sum[of \<omega> P "atrue \<Delta>"] assertify_bexp_def
+            by (smt (verit) Int_iff commutative greater_equiv mem_Collect_eq)
+          then have "\<not> bdenot b (get_store |p| )"
+            by (simp add: core_charact(1) full_add_charact(1))
+          then have "|p| \<in> ConcreteSemantics.pure_typed \<Delta> (negate (semantify_bexp b))"
+            unfolding ConcreteSemantics.pure_typed_def semantify_bexp_def negate_def
+            by (smt (verit, del_insts) CollectD CollectI TypedEqui.typed_assertionE TypedEqui.typed_core \<open>p \<in> P\<close> asm1(2) asm1(6) core_charact(1) core_in_emp_core emp_core_def framed_by_exp_def option.collapse semantify_bexp_def)
+          then have "p \<in> P \<otimes> ConcreteSemantics.pure_typed \<Delta> (negate (semantify_bexp b))"
+            using \<open>p \<in> P\<close> core_is_smaller x_elem_set_product by blast
+          then show "\<omega> \<in> (P \<otimes> ConcreteSemantics.pure_typed \<Delta> (negate (semantify_bexp b))) \<otimes> atrue \<Delta>"
+            by (meson TypedEqui.typed_intersection TypedEqui.typed_state_axioms \<open>Some \<omega> = p \<oplus> r\<close> \<open>\<omega> \<in> (P \<otimes> atrue \<Delta>) \<inter> assertify_bexp (Bnot b)\<close> asm1(6) atrue_self_framing_and_typed(1) greater_def in_times_atrue typed_state.typed_assertionE typed_state.typed_star)
+        qed
+      qed
     qed
   qed
 qed
 
-lemma translation_convert_proof:
-  assumes "translation_has_proof \<Delta> P C Q"
+
+lemma invariant_translate_induct:
+  assumes "wf_stmt \<Delta> C"
       and "well_typed_cmd \<Delta> C"
-  shows "\<exists>R. \<Delta> \<turnstile>CSL [P] C [Q \<otimes> R]" (* should have every assertion up_closed, and thus no R *)
+      and "ConcreteSemantics.wf_abs_stmt \<Delta> (fst (translate C))"
+      and "\<And>Cv. Cv \<in> snd (translate C) \<Longrightarrow> ConcreteSemantics.wf_abs_stmt \<Delta> Cv"
+    shows "invariant_translate \<Delta> P C Q"
   using assms
 proof (induct C arbitrary: P Q)
-  case Cskip
-  then obtain B where "ConcreteSemantics.SL_proof \<Delta> P Skip (B \<otimes> Q)"
-    unfolding translation_has_proof_def by force
-  then show ?case
-    by (metis ConcreteSemantics.SL_proof_Skip_elim RuleSkip add_set_commm)
-next
-  case (Cassign x1 x2)
-  then show ?case sorry
-next
-  case (Cread x1 x2)
-  then show ?case sorry
-next
-  case (Cwrite x1 x2)
-  then show ?case sorry
-next
-  case (Calloc r e)
-  then obtain B where "ConcreteSemantics.SL_proof \<Delta> P (Havoc r;; Inhale (full_ownership_with_val r e)) (B \<otimes> Q)"
-    unfolding translation_has_proof_def by force
-  then have "ConcreteSemantics.SL_proof \<Delta> P (Havoc r) (TypedEqui.exists_assert \<Delta> r P)
-  \<and> ConcreteSemantics.SL_proof \<Delta> (TypedEqui.exists_assert \<Delta> r P) (Inhale (full_ownership_with_val r e)) (B \<otimes> Q)
-  \<and> TypedEqui.self_framing_typed \<Delta> P"
-    by (metis ConcreteSemantics.SL_proof_Havoc_elim ConcreteSemantics.SL_proof_Seq_elim)
-  then have "B \<otimes> Q = TypedEqui.exists_assert \<Delta> r P \<otimes> full_ownership_with_val r e"
-    by blast
-
-  have "\<Delta> \<turnstile>CSL [UNIV \<otimes> TypedEqui.exists_assert \<Delta> r P] Calloc r e [full_ownership_with_val r e \<otimes> TypedEqui.exists_assert \<Delta> r P]"
-  proof (rule RuleFrame)
-    have "r \<notin> fvE e" sorry (* should come from well-definedness *)
-    then show "\<Delta> \<turnstile>CSL [UNIV] Calloc r e [full_ownership_with_val r e]"
-      using RuleAlloc[of r e] by simp
-    show "disjoint (fvA (TypedEqui.exists_assert \<Delta> r P)) (wrC (Calloc r e))" sorry (* Should come from fvA *)
-    show "TypedEqui.self_framing_typed \<Delta> UNIV"
-      using TypedEqui.self_framing_typed_def by blast
-    show "TypedEqui.self_framing_typed \<Delta> (TypedEqui.exists_assert \<Delta> r P)"
-      using \<open>ConcreteSemantics.SL_proof \<Delta> P (abs_stmt.Havoc r) (TypedEqui.exists_assert \<Delta> r P) \<and> ConcreteSemantics.SL_proof \<Delta> (TypedEqui.exists_assert \<Delta> r P) (abs_stmt.Inhale (full_ownership_with_val r e)) (B \<otimes> Q) \<and> TypedEqui.self_framing_typed \<Delta> P\<close> by auto
-    show "TypedEqui.typed_assertion \<Delta> (TypedEqui.exists_assert \<Delta> r P)"
-      using \<open>ConcreteSemantics.SL_proof \<Delta> P (abs_stmt.Havoc r) (TypedEqui.exists_assert \<Delta> r P) \<and> ConcreteSemantics.SL_proof \<Delta> (TypedEqui.exists_assert \<Delta> r P) (abs_stmt.Inhale (full_ownership_with_val r e)) (B \<otimes> Q) \<and> TypedEqui.self_framing_typed \<Delta> P\<close> by blast
-    show "TypedEqui.typed_assertion \<Delta> UNIV" sorry (* TODO: Adapt to typed true *)
-  qed
-
-  moreover have "UNIV \<otimes> TypedEqui.exists_assert \<Delta> r P = P"
-    sorry (* Comes from P mono *)
-  moreover have "TypedEqui.typed_assertion \<Delta> P \<and> variables \<Delta> r \<noteq> None"
-  proof
-    show "TypedEqui.typed_assertion \<Delta> P"
-      using \<open>ConcreteSemantics.SL_proof \<Delta> P (abs_stmt.Havoc r) (TypedEqui.exists_assert \<Delta> r P) \<and> ConcreteSemantics.SL_proof \<Delta> (TypedEqui.exists_assert \<Delta> r P) (abs_stmt.Inhale (full_ownership_with_val r e)) (B \<otimes> Q) \<and> TypedEqui.self_framing_typed \<Delta> P\<close> by blast
-    show "variables \<Delta> r \<noteq> None" (* Should come from the well-typedness of the program *)
-      using Calloc.prems(2) by auto
-  qed
-  then have "entails P (TypedEqui.exists_assert \<Delta> r P)"
- (* TODO: Should work, and be given by AbstractSem *)
-    using ConcreteSemantics.SL_proof_Havoc_elim_entails[of \<Delta> P r "TypedEqui.exists_assert \<Delta> r P"]    
-    using ConcreteSemantics.exists_assert_entails by blast
-
-  then show "\<exists>R. \<Delta> \<turnstile>CSL [P] Calloc r e [Q \<otimes> R]" using RuleCons
-    by (metis \<open>B \<otimes> Q = TypedEqui.exists_assert \<Delta> r P \<otimes> full_ownership_with_val r e\<close> add_set_commm calculation(1) calculation(2))
-next
-  case (Cfree x)
-  then show ?case sorry
-next
   case (Cseq C1 C2)
-  then show ?case sorry
+  then show ?case
+    by (metis (no_types, lifting) ConcreteSemantics.wf_abs_stmt.simps(7) Un_iff fst_eqD invariant_translate_seq snd_conv translate.simps(7) well_typed_cmd_aux.simps(2) wf_stmt.simps(1))
 next
   case (Cpar P1 C1 Q1 P2 C2 Q2)
-  have "translation_has_proof \<Delta> P1 C1 Q1"
-  proof (rule translation_has_proofI)
-    show "\<exists>B. ConcreteSemantics.SL_proof \<Delta> P1 (fst (translate C1)) (B \<otimes> Q1)"
-      using has_proof_with_inhale_exhale
-
-  then obtain R1 R2 where "
-(*
-    translation_has_proof \<Delta> ?P C1 ?Q \<Longrightarrow> \<exists>R. \<turnstile>CSL [?P] C1 [?Q \<otimes> R]
-    translation_has_proof \<Delta> ?P C2 ?Q \<Longrightarrow> \<exists>R. \<turnstile>CSL [?P] C2 [?Q \<otimes> R]
-    translation_has_proof \<Delta> P {P1} C1 {Q1} || {P2} C2 {Q2} Q
-*)
-(*
-\<exists>R. \<turnstile>CSL [P] {P1} C1 {Q1} || {P2} C2 {Q2} [Q \<otimes> R]
-*)
-  then show "\<exists>R. \<turnstile>CSL [P] {P1} C1 {Q1} || {P2} C2 {Q2} [Q \<otimes> R]" sorry
+  show ?case
+  proof (rule invariant_translate_parallel[of \<Delta> C1 C2 P1 Q1 P2 Q2 P])
+    show "ConcreteSemantics.wf_abs_stmt \<Delta> (ConcreteSemantics.havoc_list (wrL C1 @ wrL C2))"
+      using Cpar.prems(3) by fastforce
+    show "wf_stmt \<Delta> {P1} C1 {Q1} || {P2} C2 {Q2}"
+      using Cpar.prems(1) by blast
+    fix P Q
+    show "invariant_translate \<Delta> P C1 Q"
+    proof (rule Cpar(1))
+      have "ConcreteSemantics.wf_abs_stmt \<Delta> (Inhale P1;; fst (translate C1);; Exhale Q1)"
+        by (metis Cpar.prems(4) Un_iff insertCI snd_eqD translate.simps(9))
+      then show "ConcreteSemantics.wf_abs_stmt \<Delta> (fst (translate C1))"
+        by force
+      show "\<And>Cv. Cv \<in> snd (translate C1) \<Longrightarrow> ConcreteSemantics.wf_abs_stmt \<Delta> Cv"
+        by (metis Cpar.prems(4) Un_iff snd_eqD translate.simps(9))
+      show "well_typed_cmd \<Delta> C1"
+        using Cpar.prems(2) by auto
+      show "wf_stmt \<Delta> C1"
+        using Cpar.prems(1) by auto
+    qed
+    show "invariant_translate \<Delta> P C2 Q"
+    proof (rule Cpar(2))
+      have "ConcreteSemantics.wf_abs_stmt \<Delta> (Inhale P2;; fst (translate C2);; Exhale Q2)"
+        by (metis Cpar.prems(4) Un_iff insertCI snd_eqD translate.simps(9))
+      then show "ConcreteSemantics.wf_abs_stmt \<Delta> (fst (translate C2))"
+        by force
+      show "\<And>Cv. Cv \<in> snd (translate C2) \<Longrightarrow> ConcreteSemantics.wf_abs_stmt \<Delta> Cv"
+        by (metis Cpar.prems(4) Un_iff snd_eqD translate.simps(9))
+      show "well_typed_cmd \<Delta> C2"
+        using Cpar.prems(2) by auto
+      show "wf_stmt \<Delta> C2"
+        using Cpar.prems(1) by auto
+    qed
+  qed
 next
-  case (Cif x1 C1 C2)
-  then show ?case sorry
+  case (Cif b C1 C2)
+  show ?case
+  proof (rule invariant_translate_if[of \<Delta> C1 C2 P b ])
+    fix P Q
+    show "invariant_translate \<Delta> P C1 Q"
+    proof (rule Cif(1))
+      show "wf_stmt \<Delta> C1"
+        using Cif.prems(1) by auto
+      show "well_typed_cmd \<Delta> C1"
+        using Cif.prems(2) by auto
+      show "ConcreteSemantics.wf_abs_stmt \<Delta> (fst (translate C1))"
+        using Cif.prems(3) by fastforce
+      show "\<And>Cv. Cv \<in> snd (translate C1) \<Longrightarrow> ConcreteSemantics.wf_abs_stmt \<Delta> Cv"
+        by (metis Cif.prems(4) Un_iff snd_eqD translate.simps(8))
+    qed
+    show "invariant_translate \<Delta> P C2 Q"
+    proof (rule Cif(2))
+      show "wf_stmt \<Delta> C2"
+        using Cif.prems(1) by auto
+      show "well_typed_cmd \<Delta> C2"
+        using Cif.prems(2) by auto
+      show "ConcreteSemantics.wf_abs_stmt \<Delta> (fst (translate C2))"
+        using Cif.prems(3) by fastforce
+      show "\<And>Cv. Cv \<in> snd (translate C2) \<Longrightarrow> ConcreteSemantics.wf_abs_stmt \<Delta> Cv"
+        by (metis Cif.prems(4) Un_iff snd_eqD translate.simps(8))
+    qed
+  qed
 next
   case (Cwhile x1 C)
   then show ?case sorry
+qed (simp_all add: invariant_translate_skip invariant_translate_free invariant_translate_alloc invariant_translate_seq
+      invariant_translate_write invariant_translate_read invariant_translate_assign)
+
+
+theorem sound_translation:
+  assumes "wf_stmt \<Delta> C"
+      and "well_typed_cmd \<Delta> C"
+      and "ConcreteSemantics.wf_abs_stmt \<Delta> (fst (translate C))"
+      and "\<And>Cv. Cv \<in> snd (translate C) \<Longrightarrow> ConcreteSemantics.wf_abs_stmt \<Delta> Cv"
+      and "TypedEqui.wf_assertion \<Delta> P \<and> TypedEqui.wf_assertion \<Delta> Q"
+      and "ConcreteSemantics.self_framing_and_typed \<Delta> P \<and> TypedEqui.typed_assertion \<Delta> P"
+
+      and "ConcreteSemantics.verifies_set \<Delta> (atrue \<Delta>) (Inhale P;; fst (translate C);; Exhale Q)"
+      and "\<And>Cv. Cv \<in> snd (translate C) \<Longrightarrow> ConcreteSemantics.verifies_set \<Delta> (atrue \<Delta>) Cv"
+    shows "\<Delta> \<turnstile>CSL [P \<otimes> atrue \<Delta>] C [Q \<otimes> atrue \<Delta>]"
+proof -
+  obtain B where "ConcreteSemantics.SL_proof \<Delta> (atrue \<Delta>) (Inhale P;; fst (translate C);; Exhale Q) B"
+    by (metis ConcreteSemantics.Viper_implies_SL_proof ConcreteSemantics.wf_abs_stmt.simps(2) ConcreteSemantics.wf_abs_stmt.simps(3) ConcreteSemantics.wf_abs_stmt.simps(7) assms(3) assms(5) assms(7) atrue_self_framing_and_typed(1) atrue_self_framing_and_typed(2))
+  then obtain B' where "ConcreteSemantics.SL_proof \<Delta> (atrue \<Delta> \<otimes> P) (fst (translate C)) B'" "entails B' (B \<otimes> Q)"
+    by blast
+
+
+  show "\<Delta> \<turnstile>CSL [P \<otimes> atrue \<Delta>] C [Q \<otimes> atrue \<Delta>]"
+  proof (rule RuleCons)
+    show "\<Delta> \<turnstile>CSL [P \<otimes> atrue \<Delta> \<otimes> atrue \<Delta>] C [B' \<otimes> atrue \<Delta>]"
+    proof (rule invariant_translateE[of \<Delta> "P \<otimes> atrue \<Delta>" C])
+      show "ConcreteSemantics.SL_proof \<Delta> (P \<otimes> atrue \<Delta>) (fst (translate C)) B'"
+        by (metis \<open>ConcreteSemantics.SL_proof \<Delta> (atrue \<Delta> \<otimes> P) (fst (translate C)) B'\<close> add_set_commm)
+      show "invariant_translate \<Delta> (P \<otimes> atrue \<Delta>) C B'"
+        by (simp add: assms(1) assms(2) assms(3) assms(4) invariant_translate_induct)
+      show "proof_obligations_valid \<Delta> (snd (translate C))"
+        unfolding proof_obligations_valid_def
+      proof clarify
+        fix Cv assume "Cv \<in> snd (translate C)"
+        then show "\<exists>B. ConcreteSemantics.SL_proof \<Delta> (atrue \<Delta>) Cv B"
+          by (simp add: ConcreteSemantics.Viper_implies_SL_proof assms(4) assms(8))
+      qed
+    qed
+    show "P \<otimes> atrue \<Delta> \<subseteq> P \<otimes> atrue \<Delta> \<otimes> atrue \<Delta>"
+      by (simp add: add_set_asso atrue_twice_equal)
+    show "B' \<otimes> atrue \<Delta> \<subseteq> Q \<otimes> atrue \<Delta>"
+      by (meson ConcreteSemantics.proof_then_typed \<open>ConcreteSemantics.SL_proof \<Delta> (atrue \<Delta>) (abs_stmt.Inhale P ;; fst (translate C) ;; abs_stmt.Exhale Q) B\<close> \<open>entails B' (B \<otimes> Q)\<close> add_set_mono drop_conjunct_entails dual_order.trans entails_def order_refl)
+  qed
 qed
 
 
+(* DONE:
+- Skip
+- Assign
+- Alloc
+- Free
+- Write
+- Read
+- Seq
+- Parallel rule
 
-lemma parallel_translation_correct:
-  assumes "translation_has_proof \<Delta> ({P1} C1 {Q1} || {P2} C2 {Q2})"
-  shows "\<exists>B. \<turnstile>CSL [P] C [B "
-  sorry
+Missing:
+Compositional stuff
+\<longrightarrow> While loop
+\<longrightarrow> If
 
-
-(*
-| RulePar: "\<lbrakk> disjoint (fvC C1 \<union> fvA Q1) (wrC C2); disjoint (fvC C2 \<union> fvA Q2) (wrC C1); self_framing P1; self_framing P2;
-    \<turnstile>CSL [P1] C1 [Q1]; \<turnstile>CSL [P2] C2 [Q2] \<rbrakk> \<Longrightarrow> \<turnstile>CSL [P1 \<otimes> P2] C1 || C2 [Q1 \<otimes> Q2]"
+datatype cmd =
+| Cif bexp cmd cmd
+| Cwhile bexp cmd
 *)
+
 
 
 end
